coq-osiris/theories/program_logic/wp_step.v
@@ -9,35 +9,39 @@ Section wp_step.
 
   Context {Σ : gFunctors}.
 
-  (* Flag stating whether a thread has terminated or not. *)
-  Inductive thread_state :=
-  | Alive : thread_state
-  | Dead : outcome2 val exn -> thread_state.
+  Definition is_outcome {A X} (m : micro A X) :=
+    match m with
+    | Ret v => Some (O2Ret v)
+    | Throw v => Some (O2Throw v)
+    | _ => None
+    end.
 
-  Definition threadpool : Type := gmap thread thread_state.
-  Definition posts : Type := gmap thread (outcome2 val exn -> iProp Σ).
-
-  Definition th_config A X : Type := store * threadpool * micro A X * thread.
-  Definition th_config_step A X : Type := store * threadpool * micro A X * list (thread * microvx).
+  Definition th_config A X : Type := store * (thpool A X) * thread.
+  Definition th_config_step A X : Type := store * (thpool A X) * list (thread * micro A X).
 
   Inductive wp_step : ∀ A X, th_config A X -> th_config_step A X -> Prop :=
-  | BaseS : ∀ {A X} (m : micro A X) σ m' σ' π ι,
+  | BaseS : ∀ {A X} (m : micro A X) σ m' σ' (π : thpool A X) ι,
+      π !! ι = Some m ->
       step (σ, m) (σ', m') ->
-      wp_step A X (σ, π, m, ι) (σ', π, m', [])
-  | ForkS : ∀ {A X} σ π ι v1 v2 (k : outcome2 val exn -> micro A X) ι',
+      wp_step A X (σ, π, ι) (σ', <[ ι := m' ]> π, [])
+  | ForkS : ∀ σ π ι v1 v2 (k : outcome2 val exn -> micro val exn) ι',
+      π !! ι = Some (Stop CFork (v1, v2) k) ->
       π !! ι' = None ->
-      wp_step A X
-        (σ, π, (Stop CFork (v1, v2) k), ι)
-        (σ, <[ ι' := Alive ]> π, continue k (VThread ι'), [(ι', call v1 v2)])
-  | JoinS : ∀ {A X} σ π ι (k : outcome2 val exn -> micro A X) o ι',
-      π !! ι' = Some (Dead o) ->
-      wp_step A X
-        (σ, π, Stop CJoin ι' k, ι)
-        (σ, π, k o, [])
+      wp_step val exn
+        (σ, π, ι)
+        (σ, @insert _ _ _ insert_thpool ι' (call v1 v2)
+              (@insert _ _ _ insert_thpool ι (continue k (VThread ι')) π), [(ι', call v1 v2)])
+  | JoinS : ∀ σ (π : thpool val exn) ι (k : outcome2 val exn -> micro val exn) o ι',
+      π !! ι = Some (Stop CJoin ι' k) ->
+      (@lookup _ _ _ lookup_thpool ι' π) ≫= is_outcome = Some o ->
+      wp_step val exn
+        (σ, π, ι)
+        (σ, <[ ι := k o ]> π, [])
   | SelfS : ∀ {A X} σ π ι u (k : outcome2 val exn -> micro A X),
+      π !! ι = Some (Stop CSelf u k) ->
       wp_step A X
-        (σ, π, Stop CSelf u k, ι)
-        (σ, π, continue k (VThread ι), [])
+        (σ, π, ι)
+        (σ, <[ ι := continue k (VThread ι) ]> π, [])
   .
 
   Global Arguments wp_step {A X}.
@@ -58,6 +62,11 @@ Ltac destruct_wp_step :=
                     dependent destruction h
   end;
   try destruct_step;
+  lazymatch goal with
+    h1: ?π !! ?ι = Some ?m, h2: ?π !! ?ι = Some ?m' |- _ =>
+      rewrite h2 in h1; try discriminate h1; inversion_clear h1;
+      try (subst m || subst m')
+  end;
   (* We will often conclude that the list of forked threads is empty. *)
   try rewrite bi.sep_emp.
 
@@ -70,30 +79,41 @@ Section can_progress.
 
   Definition can_progress {A E} (c : th_config A E) :=
     match c with
-    | (_, π, Stop CJoin ι' k, _) => ι' ∈ dom π
-    | _ => ∃ c', wp_step c c'
-  end.
+    | (_, π, ι) =>
+        match π !! ι with
+        | Some (Stop CJoin ι' k) => ι' ∈ dom π
+        | Some _ => ∃ c', wp_step c c'
+        | None => False
+        end
+    end.
 
-  Lemma invert_can_progress {A E} σ π m ι :
-    @can_progress A E (σ, π, m, ι) ->
-    (∃ ι' k, m = Stop CJoin ι' k ∧ ι' ∈ dom π) ∨
+  Lemma invert_can_progress {A E} σ π ι :
+    @can_progress A E (σ, π, ι) ->
+    ∃ m, π !! ι = Some m ∧
+    ((∃ ι' k, m = Stop CJoin ι' k ∧ ι' ∈ dom π) ∨
       (∃ v1 v2 k, m = Stop CFork (v1, v2) k) ∨
       (∃ u k, m = Stop CSelf u k) ∨
-      (can_step (σ, m)).
+      (can_step (σ, m))).
   Proof.
     intros Hcp.
+    unfold can_progress in Hcp.
+    case (π !! ι) eqn:Hlookup in Hcp; last contradiction.
+    exists m; split; [ assumption | ].
     (* Cases on the micro computation. *)
     destruct m;
       (* If that computation is a Stop, destruct the code *)
       try destruct_code;
       (* Generally try to invert Hcp *)
       try (
-          destruct Hcp as ([[[??]?]?] & Hcp);
+          destruct Hcp as ([[σ' π'] ι'] & Hcp);
           dependent destruction Hcp;
+          rewrite Hlookup in H;
+          inversion H; subst;
           destruct_step; auto with step can_step);
       (* There remains some cases *)
       try solve [(do 3 right; auto with step can_step)].
-    (* Only the [Stop] case is left. *)
+
+    (* Only the concurrent [Stop] cases are left. *)
     - right; left. destruct x. repeat eexists.
     - left. repeat eexists. apply Hcp.
     - right; right; left. repeat eexists; apply Hcp.
@@ -103,78 +123,99 @@ Section can_progress.
 
   Lemma can_step_can_progress {A E} σ (m : micro A E) :
     ∀ π ι,
+      π !! ι = Some m ->
       can_step (σ, m) ->
-      can_progress (σ, π, m, ι).
+      can_progress (σ, π, ι).
   Proof.
-    intros π ι ([σ' m'] & Hstep).
+    intros π ι Hlookup ([σ' m'] & Hstep).
+    unfold can_progress; rewrite Hlookup.
     destruct_step;
-      eexists (_, π, _, []);
-      by (apply BaseS; eauto with step can_step).
+      eexists (_, <[ ι := _ ]> π, []);
+      by (eapply BaseS; eauto with step can_step).
     Unshelve. apply b.
   Qed.
 
-  Lemma can_progress_fork {A E} σ π x (k : _ -> micro A E) ι :
-    can_progress (σ, π, (Stop CFork x k), ι).
+  Lemma can_progress_fork σ π x (k : _ -> micro val exn) ι :
+    π !! ι = Some (Stop CFork x k) ->
+    can_progress (σ, π, ι).
   Proof.
+    intros Hlookup.
     destruct x.
     assert (exists ι', π !! ι' = None) as [ι' Hι'].
     { exists (fresh (dom π)).
-      apply fin_map_dom.not_elem_of_dom_1.
+      apply (fin_map_dom.not_elem_of_dom_1 π (fresh (dom π))).
       apply fin_sets.is_fresh. }
-    eexists. apply (ForkS (A:=A) (X:=E)).
-    apply Hι'.
+    unfold can_progress; rewrite Hlookup.
+    eexists. eapply ForkS; eassumption.
   Qed.
 
-  Lemma can_progress_join {A E} σ π ι' (k : _ -> micro A E) ι s :
+  Lemma can_progress_join σ π ι' (k : _ -> micro val exn) ι s :
+    π !! ι = Some (Stop CJoin ι' k) ->
     π !! ι' = Some s ->
-    can_progress (σ, π, (Stop CJoin ι' k), ι).
+    can_progress (σ, π, ι).
   Proof.
-    intros Hπ; simpl.
-    apply elem_of_dom.
+    intros Hlookup Hπ; simpl.
+    unfold can_progress; rewrite Hlookup.
+    apply (elem_of_dom π ι').
     exists s; assumption.
   Qed.
 
   Lemma inv_can_progress_join {A E} σ π ι' (k : _ -> micro A E) ι :
-    can_progress (σ, π, (Stop CJoin ι' k), ι) ->
+    π !! ι = Some (Stop CJoin ι' k) ->
+    can_progress (σ, π, ι) ->
     ∃ s, π !! ι' = Some s.
   Proof.
-    intros Hprog; simpl.
-    apply elem_of_dom.
+    intros Hlookup Hprog; simpl.
+    apply (elem_of_dom π ι').
+    unfold can_progress in Hprog; rewrite Hlookup in Hprog.
     apply Hprog.
   Qed.
 
   Lemma can_progress_self {A E} σ π u (k : _ -> micro A E) ι :
-    can_progress (σ, π, (Stop CSelf u k), ι) .
+    π !! ι = Some (Stop CSelf u k) ->
+    can_progress (σ, π, ι) .
   Proof.
-    destruct π.
-    eexists; apply SelfS.
+    intros Hlookup.
+    unfold can_progress; rewrite Hlookup.
+    eexists; apply SelfS with (u := u); eauto.
   Qed.
 
   Lemma invert_wp_step_resume {A E : Type} (σ σ' : store) π π' ι μ (l : loc) (o : outcome2 val exn)
     (k : outcome2 val exn → micro A E)
-    (sk : outcome2 val exn → microvx) (m' : micro A E) :
+    (sk : outcome2 val exn → microvx) :
+    π !! ι = Some (Stop CResume (l, o) k) ->
     σ !! l = Some (K sk) →
-    @wp_step A E (σ, π, Stop CResume (l, o) k, ι) (σ', π', m', μ) →
-    σ' = <[l:=Shot]> σ ∧ m' = try2 (sk o) k ∧ π' = π ∧ μ = [].
+    @wp_step A E (σ, π, ι) (σ', π', μ) →
+      σ' = <[l:=Shot]> σ ∧
+      π' = <[ ι := try2 (sk o) k ]> π ∧
+      μ = [].
   Proof.
-    intros Hlookup Hstep.
-    destruct_wp_step.
+    intros Hlookup' Hlookup Hstep.
+    dependent destruction Hstep;
+    rewrite H in Hlookup';
+    inversion Hlookup'; subst m.
+    destruct_step.
     repeat split; auto.
-    by unfold step_resume_1; rewrite Hlookup.
-    by unfold step_resume_2; rewrite Hlookup.
+    - unfold step_resume_1. rewrite Hlookup. reflexivity.
+    - unfold step_resume_2. rewrite Hlookup. reflexivity.
   Qed.
 
   Lemma invert_can_step_wp_step {A E} σ π (m : micro A E) ι π' m' μ σ' :
-    @wp_step A E (σ, π, m, ι) (σ', π', m', μ) ->
+    π !! ι = Some m ->
+    π' !! ι = Some m' ->
+    @wp_step A E (σ, π, ι) (σ', π', μ) ->
     can_step (σ, m) ->
     step (σ, m) (σ', m') ∧
-      π = π' ∧
+      π' = <[ ι := m' ]> π ∧
       μ = [].
   Proof.
-    intros Hwpstep Hstep.
-    destruct_wp_step; repeat constructor; auto; try solve [ exfalso; eauto with invert_can_step ].
-    eapply StepWrap; [ eassumption | reflexivity ].
-    eapply StepShallowWrap; [ eassumption | reflexivity ].
+    intros Hlookup Hlookup' Hwpstep Hstep.
+    dependent destruction Hwpstep;
+      rewrite H in Hlookup; inversion Hlookup; subst m;
+      try solve [ exfalso; eauto with invert_can_step ].
+    rewrite lookup_insert in Hlookup'. inversion Hlookup'; subst m'0.
+    clear Hlookup Hstep Hlookup'.
+    done.
   Qed.
 
   Local Ltac invert_try2 :=
@@ -182,16 +223,33 @@ Section can_progress.
     | h: step (_, try2 _ _) (_, _) |- _ => apply invert_step_try2 in h as (? & ? & ->)
     end.
 
-  Lemma invert_wp_step_try2 {A B E' E} σ π m (k : outcome2 A E' -> micro B E) ι σ' π' m' μ :
-    @wp_step B E (σ, π, try2 m k, ι) (σ', π', m', μ) ->
+  Lemma invert_wp_step_try2 {A B E' E} σ π m m' (k : outcome2 A E' -> micro B E) ι σ' π' μ :
+    π !! ι = Some (try2 m k) ->
+    π' !! ι = Some m' ->
+    @wp_step B E (σ, π, ι) (σ', π', μ) ->
     can_step (σ, m) ->
-    ∃ m'', @wp_step A E' (σ, π, m, ι) (σ', π, m'', []) ∧ m' = try2 m'' k.
+    ∃ m'', m' = try2 m'' k.
   Proof.
-    intros Hwp Hstep.
-    destruct m; intros;
-      destruct_wp_step;
-      try solve [ exfalso; eauto with invert_can_step ];
-      eexists; (split; [ apply BaseS; eauto with step | eauto with try2_algebraic try_try ]).
+    intros Hlookup Hlookup' Hwp Hstep.
+    dependent destruction Hwp;
+      rewrite H in Hlookup; inversion Hlookup; subst;
+      try solve [ exfalso; eauto with invert_can_step ].
+    { apply invert_step_try2 in H0; last assumption.
+      destruct H0 as (? & Hstep' & ->).
+      rewrite lookup_insert in Hlookup'; inversion Hlookup'; subst.
+      eexists; reflexivity. }
+    - symmetry in H2.
+      apply invert_try2_eq_stop in H2 as (k' & -> & ->);
+        try (intros ? ->);
+      exfalso; eauto with invert_can_step.
+    - symmetry in H2.
+      apply invert_try2_eq_stop in H2 as (k' & -> & ->);
+        try (intros ? ->);
+        exfalso; eauto with invert_can_step.
+    - symmetry in H1.
+      apply invert_try2_eq_stop in H1 as (k' & -> & ->);
+        try (intros ? ->);
+        exfalso; eauto with invert_can_step.
   Qed.
 
 End can_progress.
